theories/lang.v
@@ -10,6 +10,7 @@ From iris.proofmode Require Import tactics.
 
 (* Helper tactics *)
 Ltac inv H := inversion H; subst; clear H.
+Ltac rw_inj H0 H1 := rewrite H0 in H1; injection H1; intros; subst; clear H1.
 
 Definition tag := string.
 
@@ -87,15 +88,73 @@ Section nested_ind.
     end.
 End nested_ind.
 
+(* Not used yet *)
+Inductive bounded (n: nat) : lang_ty → Prop :=
+  | ClassIsBounded cname targs :
+      Forall (bounded n) targs → bounded n (ClassT cname targs)
+  | UnionIsBounded s t :
+      bounded n s → bounded n t → bounded n (UnionT s t)
+  | InterIsBounded s t :
+      bounded n s → bounded n t → bounded n (InterT s t)
+  | GenIsBounded k:
+      k < n → bounded n (GenT k)
+  | IntIsBounded : bounded n IntT
+  | BoolIsBounded : bounded n BoolT
+  | NothingIsBounded : bounded n NothingT
+  | MixedIsBounded : bounded n MixedT
+  | NullIsBounded : bounded n NullT
+  | NonNullIsBounded : bounded n NonNullT
+  | ExIsBounded cname : bounded n (ExT cname)
+.
+
+Global Hint Constructors bounded : core.
+
 (* Generics must be always bound *)
 Fixpoint subst_ty (targs:list lang_ty) (ty: lang_ty):  lang_ty :=
   match ty with
-  | ClassT cname cargs => ClassT cname (map (subst_ty targs) cargs)
+  | ClassT cname cargs => ClassT cname (subst_ty targs <$> cargs)
   | UnionT s t => UnionT (subst_ty targs s) (subst_ty targs t)
   | InterT s t => InterT (subst_ty targs s) (subst_ty targs t)
   | GenT n => default NothingT (targs !! n)
   | ExT _ | IntT | BoolT | NothingT | MixedT | NullT | NonNullT => ty
   end.
+
+Lemma subst_ty_subst ty l k:
+  subst_ty l (subst_ty k ty) = subst_ty (subst_ty l <$> k) ty.
+Proof.
+  induction ty as [ | | | | cname targs hi | | | s t hs ht |
+      s t hs ht | n | cname ] => //=.
+  - f_equal.
+    rewrite -list_fmap_compose.
+    rewrite Forall_forall in hi.
+    apply map_ext_in => s /elem_of_list_In hin.
+    by apply hi.
+  - by f_equal.
+  - by f_equal.
+  - destruct (k !! n) as [ ty | ] eqn:hty.
+    + by rewrite /= list_lookup_fmap hty.
+    + by rewrite /= list_lookup_fmap hty.
+Qed.
+
+Lemma map_subst_ty_subst (j k l: list lang_ty):
+  subst_ty j <$> (subst_ty k <$> l) =
+  subst_ty (subst_ty j <$> k) <$> l.
+Proof.
+  induction l as [ | hd tl hi] => //=.
+  rewrite subst_ty_subst.
+  f_equal.
+  by rewrite list_fmap_compose -/subst_ty list_fmap_id -/fmap hi.
+Qed.
+
+Lemma fmap_subst_ty_subst j k (l: stringmap lang_ty):
+  subst_ty j <$> (subst_ty k <$> l) =
+  subst_ty (subst_ty j <$> k) <$> l.
+Proof.
+  move: j k.
+  induction l as [| s ty ftys Hs IH] using map_ind => j k;
+    first by rewrite !fmap_empty.
+  by rewrite !fmap_insert subst_ty_subst IH.
+Qed.
 
 Definition var := string.
 Global Instance var_dec_eq (l l' : var) : Decision (l = l') := _.
@@ -118,7 +177,7 @@ Inductive cmd : Set :=
   | LetC (lhs: var) (e: expr)
   | IfC (cond: expr) (thn: cmd) (els: cmd)
   | CallC (lhs: var) (recv: expr) (name: string) (args: stringmap expr)
-  | NewC (lhs: var) (class_name: tag) (targs: list lang_ty) (args: stringmap expr)
+  | NewC (lhs: var) (class_name: tag) (args: stringmap expr)
   | GetC (lhs: var) (recv: expr) (name: string)
   | SetC (recv: expr) (fld: string) (rhs: expr)
       (* tag test "if ($v is C) { ... }" *)
@@ -133,19 +192,50 @@ Record methodDef := {
   methodret: expr;
 }.
 
+Definition subst_mdef targs mdef : methodDef := {|
+    methodname := mdef.(methodname);
+    methodargs := subst_ty targs <$> mdef.(methodargs);
+    methodrettype := subst_ty targs mdef.(methodrettype);
+    methodbody := mdef.(methodbody);
+    methodret := mdef.(methodret);
+  |}.
+
+Lemma subst_mdef_mdef k l mdef :
+  subst_mdef k (subst_mdef l mdef) = subst_mdef (subst_ty k <$> l) mdef.
+Proof.
+  rewrite /subst_mdef; destruct mdef as [? args ret ? ?]; f_equiv => //=.
+  - by rewrite fmap_subst_ty_subst.
+  - by rewrite subst_ty_subst.
+Qed.
+
+
 Record classDef := {
   classname: tag;
   generics: nat; (* number of generics, no constraint for now *)
-  superclass: option tag;
+  superclass: option (tag * list lang_ty);
   classfields : stringmap lang_ty;
   classmethods : stringmap methodDef;
 }.
 
+(* Wf defintions on the source *)
+Definition mdef_bounded n mdef : Prop :=
+  map_Forall (λ _argname, bounded n) mdef.(methodargs) ∧ bounded n mdef.(methodrettype).
+
+Definition cdef_methods_bounded cdef : Prop :=
+  map_Forall (λ _mname mdef, mdef_bounded cdef.(generics) mdef) cdef.(classmethods).
+
+(* "Identity" substitution for n generics *)
 Fixpoint gen_targs_ nleft n : list lang_ty :=
   match nleft with
   | O => []
   | S nleft => GenT n :: gen_targs_ nleft (S n)
   end.
+
+Lemma length_gen_targs_: ∀ nleft n, length (gen_targs_ nleft n) = nleft.
+Proof.
+  elim => [ | nleft hi] n //=.
+  by rewrite hi.
+Qed.
 
 Lemma lookup_gen_targs__lt :
   ∀ nleft n pos, pos < nleft →
@@ -188,6 +278,66 @@ Proof.
   by rewrite lookup_gen_targs__ge.
 Qed.
 
+Corollary length_gen_targs n : length (gen_targs n) = n.
+Proof. by rewrite /gen_targs length_gen_targs_. Qed.
+
+Corollary gen_targs_O : gen_targs 0 = [].
+Proof. done. Qed.
+
+Lemma subst_gen_targs_is_bounded n ty:
+  bounded n ty →
+  subst_ty (gen_targs n) ty = ty.
+Proof.
+  move => h.
+  induction ty as [ | | | | cname targs hi | | | s t hs ht |
+      s t hs ht | k | cname ] => //=.
+  - f_equal.
+    rewrite Forall_forall in hi.
+    pattern targs at 2.
+    replace targs with (map id targs) by apply map_id.
+    apply map_ext_in => /= s /elem_of_list_In hin.
+    apply hi => //.
+    inv h.
+    rewrite Forall_forall in H0.
+    by apply H0.
+  - inv h; f_equal; by eauto.
+  - inv h; f_equal; by eauto.
+  - inv h.
+    by rewrite lookup_gen_targs_lt.
+Qed.
+
+Lemma subst_ty_gen_targs n targs :
+  length targs = n →
+  subst_ty targs <$> (gen_targs n) = targs.
+Proof.
+  move => hlen.
+  apply nth_ext with NothingT NothingT.
+  - by rewrite map_length length_gen_targs.
+  - rewrite map_length length_gen_targs => k hk.
+    rewrite !nth_lookup.
+    f_equal.
+    rewrite list_lookup_fmap lookup_gen_targs_lt => //=.
+    rewrite -hlen in hk.
+    apply lookup_lt_is_Some_2 in hk.
+    destruct (targs !! k) => //=.
+    by elim hk.
+Qed.
+
+Lemma subst_mdef_gen_targs_is_bounded n mdef :
+  mdef_bounded n mdef →
+  subst_mdef (gen_targs n) mdef = mdef.
+Proof.
+  rewrite /mdef_bounded /subst_mdef; move => [/map_Forall_lookup hargs hret].
+  rewrite subst_gen_targs_is_bounded => //.
+  replace (subst_ty (gen_targs n) <$> methodargs mdef) with (methodargs mdef);
+    first by destruct mdef.
+  apply map_eq => k.
+  rewrite lookup_fmap.
+  destruct (methodargs mdef !! k) as [ty | ] eqn:hty => //=.
+  apply hargs in hty.
+  by rewrite subst_gen_targs_is_bounded.
+Qed.
+
 (* A program is a collection of classes *)
 Class ProgDefContext := { Δ : stringmap classDef }.
 
@@ -196,42 +346,53 @@ Section ProgDef.
   (* assume a given set of class definitions *)
   Context `{PDC: ProgDefContext}.
 
-  (* class A extends B *)
-  Definition extends (A B: tag) : Prop :=
-    ∃ cdef,
-    Δ !! A = Some cdef ∧
-    cdef.(superclass) = Some B
+  (* source relation `class A<...> extends B<...>` *)
+  Inductive extends_using : tag → tag → list lang_ty → Prop :=
+    | ExtendsUsing A B cdef σB:
+        Δ !! A = Some cdef →
+        cdef.(superclass) = Some (B, σB) →
+        extends_using A B σB.
+
+  Hint Constructors extends_using : core.
+
+  Inductive extends: tag → tag → Prop :=
+    | Extends A B cdef σB:
+        Δ !! A = Some cdef →
+        cdef.(superclass) = Some (B, σB) →
+        extends A B.
+
+  Hint Constructors extends : core.
+
+  Inductive inherits_using : tag → tag → list lang_ty → Prop :=
+    | InheritsExtends A B σ:
+        extends_using A B σ →
+        inherits_using A B σ
+    | InheritsTrans A B σB C σC:
+        inherits_using A B σB →
+        inherits_using B C σC →
+        inherits_using A C (subst_ty σB <$> σC)
   .
 
-  (* Refl trans closure of extends *)
+  Hint Constructors inherits_using : core.
+
   Definition inherits := rtc extends.
 
-  (* Not useful, just for sanity check: inherits are chains.
-   * if A inherits B and C, then either B inherits C or C inherits B.
-   *)
-  Corollary inherits_is_chain:
-    ∀ A B C,
-    inherits A B → inherits A C →
-    (inherits C B ∨ inherits B C).
+  Lemma inherits_to_using A B:
+    inherits A B → (A = B) ∨ ∃ σ, inherits_using A B σ.
   Proof.
-    intros A B C h; revert C.
-    induction h as [ t | x y z hxy hyz hi]; move => c hc; first by right.
-    destruct hxy as (cdef & hin & hs).
-    destruct hc as [ t | u v w huv hvw].
-    - left; econstructor; first by exists cdef. done.
-    - destruct huv as (? & hin' & hs').
-      rewrite hin' in hin.
-      injection hin; intros ->; clear hin hin'.
-      rewrite hs' in hs.
-      injection hs; intros ->; clear hs hs'.
-      apply hi in hvw as [h | h]; first by left.
-      by right.
+    induction 1 as [ x | x y z hxy hyz hi].
+    - by left.
+    - destruct hi as [-> | [σ hi]]; right.
+      + inv hxy.
+        exists σB; by eauto.
+      + inv hxy.
+        exists (subst_ty σB <$> σ); by eauto.
   Qed.
 
   Inductive subtype : lang_ty → lang_ty → Prop :=
     | SubMixed : ∀ ty, subtype ty MixedT
-    (* Generic class are invariant *)
-    | SubClass : ∀ A B targs, inherits A B → subtype (ClassT A targs) (ClassT B targs)
+    | SubClass : ∀ A σA B σB, extends_using A B σB →
+        subtype (ClassT A σA) (ClassT B (subst_ty σA <$> σB))
     | SubMixed2: subtype MixedT (UnionT NonNullT NullT)
     | SubIntNonNull: subtype IntT NonNullT
     | SubBoolNonNull: subtype BoolT NonNullT
@@ -246,536 +407,732 @@ Section ProgDef.
     | SubRefl: ∀ s, subtype s s
     | SubTrans : ∀ s t u, subtype s t → subtype t u → subtype s u
     | SubExT : ∀ cname targs, subtype (ClassT cname targs) (ExT cname)
-    .
+  .
+  (* TODO: add Nothing <: t ? *)
 
-    Hint Constructors subtype : core.
+  Hint Constructors subtype : core.
 
-    Notation "s <: t" := (subtype s t) (at level 70, no associativity).
+  Notation "s <: t" := (subtype s t) (at level 70, no associativity).
 
-    (* Derived rules *)
-    Lemma subtype_union_comm : ∀ A B, (UnionT A B) <: (UnionT B A).
-    Proof. by auto.  Qed.
+  (* Not used yet *)
+  Inductive is_class : lang_ty → Prop :=
+    | IsClass A σA : is_class (ClassT A σA)
+  .
 
-    Lemma subtype_inter_comm : ∀ A B, (InterT A B) <: (InterT B A).
-    Proof. by auto.  Qed.
+  Lemma SubClassInherits A B σB:
+    inherits_using A B σB →
+    ∀ σA,
+    (ClassT A σA) <: (ClassT B (subst_ty σA <$> σB)).
+  Proof.
+    induction 1 as [ A B σ hext | A B σB C σC hAB hiAB hBC hiBC ] => σA (*hσA*).
+    - by econstructor.
+    - eapply SubTrans.
+      + by apply hiAB.
+      + rewrite map_subst_ty_subst.
+        by apply hiBC.
+  Qed.
 
-    Lemma subtype_union_assoc:
-      ∀ A B C, (UnionT (UnionT A B) C) <: (UnionT A (UnionT B C)).
-    Proof. by eauto.  Qed.
+  Lemma subtype_subst A B:
+    A <: B → ∀ targs, (subst_ty targs A) <: (subst_ty targs B).
+  Proof.
+    induction 1 as [ ty | A σA B σB hext | | | | A args | s t | s t
+      | s t u hs his ht hit | s t | s t | s t u hs his ht hit | s
+      | s t u hst hist htu hitu | cname args ] => targs //=.
+    - rewrite map_subst_ty_subst.
+      by constructor.
+    - constructor; by eauto.
+    - constructor; by eauto.
+    - econstructor; by eauto.
+  Qed.
 
-    Lemma subtype_inter_assoc:
-      ∀ A B C, (InterT (InterT A B) C) <: (InterT A (InterT B C)).
-    Proof. by eauto.  Qed.
+  Corollary subtype_inst_class A B σA σB σ :
+    (ClassT A σA) <: (ClassT B σB) →
+    (ClassT A (subst_ty σ <$> σA)) <: (ClassT B (subst_ty σ <$> σB)).
+  Proof.
+    move => h.
+    by apply subtype_subst with (targs := σ) in h.
+  Qed.
 
-    Definition local_tys := stringmap lang_ty.
+  (* Derived rules *)
+  Lemma subtype_union_comm : ∀ A B, (UnionT A B) <: (UnionT B A).
+  Proof. by auto.  Qed.
 
-    Definition lty_sub (lty rty: local_tys) :=
-      ∀ k A, rty !! k = Some A → ∃ B, lty !! k = Some B ∧ B <: A.
+  Lemma subtype_inter_comm : ∀ A B, (InterT A B) <: (InterT B A).
+  Proof. by auto.  Qed.
 
-    Notation "lty <:< rty" := (lty_sub lty rty) (at level 70, no associativity).
+  Lemma subtype_union_assoc:
+    ∀ A B C, (UnionT (UnionT A B) C) <: (UnionT A (UnionT B C)).
+  Proof. by eauto. Qed.
 
-    Lemma lty_sub_reflexive: reflexive _ lty_sub.
-    Proof.
-      move => lty k A ->.
-      by exists A.
-    Qed.
+  Lemma subtype_inter_assoc:
+    ∀ A B C, (InterT (InterT A B) C) <: (InterT A (InterT B C)).
+  Proof. by eauto.  Qed.
 
-    Lemma lty_sub_transitive: transitive _ lty_sub.
-    Proof.
-      move => lty rty zty hlr hrz k A hA.
-      apply hrz in hA as (C & hC & hsub).
-      apply hlr in hC as (B & -> & hsub').
-      exists B; by eauto.
-    Qed.
+  Definition local_tys := stringmap lang_ty.
 
-    (* has_field fname ty cname checks if the class cname has a field named
-     * fname of type ty
-     *)
-    Inductive has_field (fname: string) (typ: lang_ty): tag → Prop :=
-      | HasField current cdef:
-          Δ !! current = Some cdef →
-          cdef.(classfields) !! fname = Some typ →
-          has_field fname typ current
-      | InheritsField current parent cdef:
-          Δ !! current = Some cdef →
-          cdef.(classfields) !! fname = None →
-          cdef.(superclass) = Some parent →
-          has_field fname typ parent →
-          has_field fname typ current.
+  Definition lty_sub (lty rty: local_tys) :=
+    ∀ k A, rty !! k = Some A → ∃ B, lty !! k = Some B ∧ B <: A.
 
-    Hint Constructors has_field : core.
+  Notation "lty <:< rty" := (lty_sub lty rty) (at level 70, no associativity).
 
-    (* Naive method lookup: methods are unique *)
-    Inductive has_method (mname: string) (mdef: methodDef): tag → Prop :=
-      | HasMethod current cdef:
-          Δ !! current = Some cdef →
-          cdef.(classmethods) !! mname = Some mdef →
-          has_method mname mdef current
-      | InheritsMethod current parent cdef:
-          Δ !! current = Some cdef →
-          cdef.(classmethods) !! mname = None →
-          cdef.(superclass) = Some parent →
-          has_method mname mdef parent →
-          has_method mname mdef current
-    .
+  Lemma lty_sub_reflexive: reflexive _ lty_sub.
+  Proof.
+    move => lty k A ->.
+    by exists A.
+  Qed.
 
-    Hint Constructors has_method : code.
+  Lemma lty_sub_transitive: transitive _ lty_sub.
+  Proof.
+    move => lty rty zty hlr hrz k A hA.
+    apply hrz in hA as (C & hC & hsub).
+    apply hlr in hC as (B & -> & hsub').
+    exists B; by eauto.
+  Qed.
 
-    Lemma has_method_from m mdef A:
-      has_method m mdef A →
-      ∃ B cdef,
-      Δ !! B = Some cdef ∧
-      cdef.(classmethods) !! m = Some mdef ∧
-      inherits A B.
-    Proof.
-      induction 1 as [ current cdef hΔ hm | current parent cdef hΔ hm hs h hi];
-          first by exists current, cdef.
-      destruct hi as (B & cdef' & hΔ' & hm' & hinherits). 
-      exists B, cdef'; repeat split => //.
-      econstructor; last by apply hinherits.
-      by exists cdef.
-    Qed.
+  Inductive has_field (fname: string) : tag -> lang_ty → list lang_ty → Prop :=
+    | HasField tag cdef typ:
+        Δ !! tag = Some cdef →
+        cdef.(classfields) !! fname = Some typ →
+        has_field fname tag typ (gen_targs cdef.(generics))
+    | InheritsField tag targs parent inst cdef typ:
+        Δ !! tag = Some cdef →
+        cdef.(classfields) !! fname = None →
+        cdef.(superclass) = Some (parent, targs) →
+        has_field fname parent typ inst →
+        has_field fname tag typ (subst_ty targs <$> inst)
+  .
 
-    (* A class cannot redeclare a field if it is present in
-     * any of its parent definition.
-     *)
-    Definition wf_cdef_fields cdef : Prop :=
-      ∀ f fty super,
-      cdef.(superclass) = Some super →
-      has_field f fty super →
-      cdef.(classfields) !! f = None.
+  Hint Constructors has_field : core.
 
-    (* We allow method override: children can redeclare a method if types
-     * are compatible:
-     * - return type must be a subtype
-     * - argument types must be a supertype
-     *)
-    Definition mdef_incl sub super :=
-      dom stringset sub.(methodargs) = dom _ super.(methodargs) ∧
-      (∀ k A B, sub.(methodargs) !! k = Some A →
-      super.(methodargs) !! k = Some B → B <: A) ∧
-      sub.(methodrettype) <: super.(methodrettype).
+  Lemma has_field_fun fname A typ σ:
+    has_field fname A typ σ →
+    ∀ typ' σ', has_field fname A typ' σ' →
+    typ = typ' ∧ σ = σ'.
+  Proof.
+    induction 1 as [ tag cdef typ hΔ hf
+      | tag targs parent inst cdef typ hΔ hf hs h hi ] => typ' σ' h'.
+    - inv h'.
+      + rw_inj hΔ H.
+        rw_inj hf H0.
+        done.
+      + rw_inj hΔ H.
+        rewrite hf in H0; discriminate.
+    - inv h'.
+      + rw_inj hΔ H.
+        rewrite hf in H0; discriminate.
+      + rw_inj hΔ H.
+        rw_inj hs H1.
+        by apply hi in H2 as [-> ->].
+  Qed.
 
-    Lemma mdef_incl_reflexive: reflexive _ mdef_incl.
-    Proof.
-      move => mdef; split; first done.
-      split; last done.
-      by move => k A B -> [] ->.
-    Qed.
+  (* A class cannot redeclare a field if it is present in
+   * any of its parent definition.
+   *)
+  Definition wf_cdef_fields cdef : Prop :=
+    ∀ f fty σ super inst,
+    cdef.(superclass) = Some (super, inst) →
+    has_field f super fty σ →
+    cdef.(classfields) !! f = None.
 
-    Lemma mdef_incl_transitive: transitive _ mdef_incl.
-    Proof.
-      move => m0 m1 m2 [hdom1 [h1 ?]] [hdom2 [h2 ?]]; split; first by etransitivity.
-      split; last by eauto.
-      move => k A B hA hB.
-      destruct (methodargs m1 !! k) as [C | ] eqn:hC; last first.
-      { apply mk_is_Some in hA.
-        apply elem_of_dom in hA.
-        rewrite hdom1 in hA.
-        apply elem_of_dom in hA.
-        rewrite hC in hA.
-        by elim: hA.
-      }
-      apply SubTrans with C.
-      - by eapply h2.
-      - by eapply h1.
-    Qed.
+  Definition wf_cdef_fields_bounded cdef : Prop :=
+    map_Forall (λ _fname, bounded cdef.(generics)) cdef.(classfields).
 
-    Definition wf_cdef_methods cdef : Prop :=
-      ∀ m mdef superdef super,
-      cdef.(superclass) = Some super →
-      has_method m superdef super →
-      cdef.(classmethods) !! m = Some mdef →
-      mdef_incl mdef superdef.
+  (*
+  Lemma has_field_extends_using fname A typ finst:
+    map_Forall (λ _cname, wf_cdef_fields) Δ →
+    has_field fname A typ finst →
+    ∀ B σB typ' finst',
+    extends_using A B σB →
+    has_field fname B typ' finst' →
+    (typ = typ' ∧ finst = subst_ty σB <$> finst').
+  Proof.
+    move => hwf.
+    induction 1 as [ tag cdef typ hΔ hf
+      | tag targs parent inst cdef typ hΔ hf hs h hi ] => B σB typ' finst' hext hB.
+    - rewrite map_Forall_lookup in hwf.
+      inv hext.
+      rewrite hΔ in H; injection H; intros; subst; clear H.
+      apply hwf in hΔ.
+      by rewrite (hΔ _ _ _ _ _ H0 hB) in hf.
+    - inv hext.
+      rewrite hΔ in H; injection H; intros; subst; clear H.
+      rewrite hs in H0; injection H0; intros; subst; clear H0.
+      by apply (has_field_fun _ _ _ _ h) in hB as [-> ->].
+  Qed.
+  *)
 
-    (* all fields of class cname are in the fnames set *)
-    Definition has_fields (cname: tag) (fnames: stringmap lang_ty) : Prop :=
-      ∀ fname typ, has_field fname typ cname ↔ fnames !! fname = Some typ.
+  (* Naive method lookup: methods are unique. *)
+  Inductive has_method (mname: string) : methodDef → tag → Prop :=
+    | HasMethod tag cdef mdef:
+        Δ !! tag = Some cdef →
+        cdef.(classmethods) !! mname = Some mdef →
+        has_method mname mdef tag
+    | InheritsMethod tag parent σ cdef mdef:
+        Δ !! tag = Some cdef →
+        cdef.(classmethods) !! mname = None →
+        cdef.(superclass) = Some (parent, σ) →
+        has_method mname mdef parent →
+        has_method mname mdef tag
+  .
 
-    Lemma has_fields_fun: ∀ c fs0 fs1,
-      has_fields c fs0 → has_fields c fs1 → fs0 = fs1.
-    Proof.
-      move => c fs0 fs1 h0 h1.
-      apply map_eq => k.
-      destruct (fs0 !! k) as [ ty | ] eqn:hty.
-      - destruct (h1 k ty) as [hl1 hr1].
-        rewrite hl1 //=.
-        by apply h0.
-      - destruct (fs1 !! k) as [ ty | ] eqn:hty'; last done.
-        destruct (h1 k ty) as [hl1 hr1].
-        apply h0 in hr1; last done.
-        by rewrite hty in hr1.
-    Qed.
+  Hint Constructors has_method : code.
 
-    Lemma has_method_fun: ∀ c name mdef0 mdef1,
-      has_method name mdef0 c → has_method name mdef1 c → mdef0 = mdef1.
-    Proof.
-      move => c name mdef0 mdef1 h; move: mdef1.
-      induction h as [ current cdef hΔ hm | current parent cdef hΔ hm hs hp hi ].
-      - move => mdef1 h1; inv h1.
-        + rewrite hΔ in H; injection H; intros; subst; clear hΔ H.
-          rewrite hm in H0; by injection H0.
-        + rewrite hΔ in H; injection H; intros; subst; clear hΔ H.
-          rewrite hm in H0; discriminate H0.
-      - move => mdef1 h1; inv h1.
-        + rewrite hΔ in H; injection H; intros; subst; clear hΔ H.
-          rewrite hm in H0; discriminate H0.
-        + rewrite hΔ in H; injection H; intros; subst; clear hΔ H.
-          rewrite hs in H1; injection H1; intros; subst; clear hs H1.
-          by apply hi.
-    Qed.
+  (*
+  Lemma has_method_from n m mdef A:
+    mdef_bounded n mdef →
+    has_method m mdef A →
+    ∃ B cdef orig inst,
+    Δ !! B = Some cdef ∧
+    cdef.(classmethods) !! m = Some orig ∧
+    mdef = subst_mdef inst orig ∧
+    inherits A B.
+  Proof.
+    move => hwf.
+    induction 1 as [ tag cdef mdef hΔ hm 
+      | tag parent inst cdef mdef hΔ hm hs h hi].
+    - exists tag, cdef, mdef, (gen_targs n); repeat split => //.
+      by rewrite subst_mdef_gen_targs_is_bounded.
+    - destruct hi as (B & bdef & orig & Binst & hΔ' & horig & heq & hinherits). 
+      exists B, bdef, orig, (subst_ty targs <$> Binst).
+      split; first done.
+      split; first done.
+      split; first by rewrite heq subst_mdef_mdef.
+      econstructor; last first.
+      + change (ClassT B (subst_ty targs <$> Binst)) with
+        (subst_ty targs (ClassT B Binst)).
+        apply inherits_subst.
+        exact hinherits.
+      + by econstructor.
+  Qed.
+   *)
 
-    Lemma has_field_inherits : map_Forall (fun _ => wf_cdef_fields) Δ →
-      ∀ A B, inherits A B →
-      ∀ f fty, has_field f fty B → has_field f fty A.
-    Proof.
-      move => wfΔ A B h.
-      induction h as [ t | x y z hxy hyz hi]; move => f fty hf; first done.
-      apply hi in hf.
-      destruct hxy as (cdef & hΔ & hs).
-      apply InheritsField with y cdef; move => //.
-      apply wfΔ in hΔ.
-      by eapply hΔ.
-    Qed.
 
-    Corollary has_fields_inherits_lookup:
-      map_Forall (fun _ => wf_cdef_fields) Δ →
-      ∀ A B name fty fields,
-      has_field name fty B →
-      inherits A B →
-      has_fields A fields →
-      fields !! name = Some fty.
-    Proof.
-      move => wfΔ A B name fty fields hfields hinherits hf.
-      destruct (hf name fty) as [hl hr].
-      apply hl.
-      by eapply (has_field_inherits wfΔ).
-    Qed.
+  (* We allow method override: children can redeclare a method if types
+   * are compatible:
+   * - return type must be a subtype
+   * - argument types must be a supertype
+   *)
+  Definition mdef_incl sub super :=
+    dom stringset sub.(methodargs) = dom _ super.(methodargs) ∧
+    (∀ k A B, sub.(methodargs) !! k = Some A →
+    super.(methodargs) !! k = Some B → B <: A) ∧
+    sub.(methodrettype) <: super.(methodrettype).
 
-    Lemma has_method_inherits (Hcdef: map_Forall (fun _ => wf_cdef_methods) Δ):
-      ∀ A B, inherits A B →
-      ∀ m mdef, has_method m mdef B →
-      ∃ mdef', has_method m mdef' A ∧ mdef_incl mdef' mdef.
-    Proof.
-      move => A B h.
-      induction h as [ t | x y z hxy hyz hi]; move => m mdef hf.
-      { exists mdef; split => //.
-        by apply mdef_incl_reflexive.
-      }
-      apply hi in hf as (mdef' & hm & hincl).
-      destruct hxy as (cdef & hΔ & hs).
-      destruct (cdef.(classmethods) !! m) as [ mdef'' | ] eqn:heq; last first.
-      { exists mdef'; split; last done.
-        by apply InheritsMethod with y cdef.
-      }
-      exists mdef''; split; first by apply HasMethod with cdef.
-      apply mdef_incl_transitive with mdef'; last done.
-      apply Hcdef in hΔ.
-      by eapply hΔ.
-    Qed.
+  Lemma mdef_incl_reflexive: reflexive _ mdef_incl.
+  Proof.
+    move => mdef; split; first done.
+    split; last done.
+    by move => k A B -> [] ->.
+  Qed.
 
-    (* Typing Judgements *)
-    Definition is_bool_op op : bool :=
-      match op with
-      | LeqO | GeqO | EqO => true
-      | PlusO | MinusO | TimesO | DivO => false
-      end
-    .
-
-    Inductive expr_has_ty (lty : local_tys) :
-      expr → lang_ty → Prop :=
-      | IntTy : ∀ z, expr_has_ty lty (IntE z) IntT
-      | BoolTy: ∀ b, expr_has_ty lty (BoolE b) BoolT
-      | NullTy: expr_has_ty lty NullE NullT
-      | OpIntTy: ∀ op e1 e2,
-          is_bool_op op = false →
-          expr_has_ty lty e1 IntT →
-          expr_has_ty lty e2 IntT →
-          expr_has_ty lty (OpE op e1 e2) IntT
-      | OpBoolTy: ∀ op e1 e2,
-          is_bool_op op = true →
-          expr_has_ty lty e1 IntT →
-          expr_has_ty lty e2 IntT →
-          expr_has_ty lty (OpE op e1 e2) BoolT
-      | GenTy: ∀ v ty,
-          lty !! v = Some ty →
-          expr_has_ty lty (VarE v) ty
-      | ESubTy: ∀ e s t,
-          expr_has_ty lty e s →
-          s <: t →
-          expr_has_ty lty e t
-    .
-
-    (* continuation-based typing for commands *)
-    Inductive cmd_has_ty :
-      local_tys → cmd → local_tys → Prop :=
-      | SkipTy: ∀ lty, cmd_has_ty lty SkipC lty
-      | SeqTy: ∀ lty1 lty2 lty3 fstc sndc,
-          cmd_has_ty lty1 fstc lty2 →
-          cmd_has_ty lty2 sndc lty3 →
-          cmd_has_ty lty1 (SeqC fstc sndc) lty3
-      | LetTy: ∀ lty lhs e ty,
-          expr_has_ty lty e ty →
-          cmd_has_ty lty (LetC lhs e) (<[lhs := ty]>lty)
-      | IfTy: ∀ lty1 lty2 cond thn els,
-          expr_has_ty lty1 cond BoolT →
-          cmd_has_ty lty1 thn lty2 →
-          cmd_has_ty lty1 els lty2 →
-          cmd_has_ty lty1 (IfC cond thn els) lty2
-      | GetTy: ∀ lty lhs recv t targs name fty,
-          expr_has_ty lty recv (ClassT t targs) →
-          has_field name fty t →
-          cmd_has_ty lty (GetC lhs recv name) (<[lhs := subst_ty targs fty]>lty)
-      | SetTy: ∀ lty recv fld rhs fty t targs,
-          expr_has_ty lty recv (ClassT t targs) →
-          has_field fld fty t →
-          expr_has_ty lty rhs (subst_ty targs fty) →
-          cmd_has_ty lty (SetC recv fld rhs) lty
-      | NewTy: ∀ lty lhs t targs args fields,
-          has_fields t fields →
-          dom (gset string) fields = dom _ args →
-          (∀ f fty arg,
-          fields !! f = Some fty →
-          args !! f = Some arg →
-          expr_has_ty lty arg (subst_ty targs fty)) →
-          cmd_has_ty lty (NewC lhs t targs args) (<[ lhs := ClassT t targs]>lty)
-      | CallTy: ∀ lty lhs recv t targs name mdef args,
-          expr_has_ty lty recv (ClassT t targs) →
-          has_method name mdef t →
-          dom (gset string) mdef.(methodargs) = dom _ args →
-          (∀ x ty arg,
-          mdef.(methodargs) !! x = Some ty →
-          args !! x = Some arg →
-          expr_has_ty lty arg (subst_ty targs ty)) →
-          cmd_has_ty lty (CallC lhs recv name args) (<[lhs := subst_ty targs mdef.(methodrettype)]>lty)
-      | SubTy: ∀ lty c rty rty',
-          rty' <:< rty →
-          cmd_has_ty lty c rty' →
-          cmd_has_ty lty c rty
-      | CondTagTy lty v tv t cmd :
-          lty !! v = Some tv →
-          cmd_has_ty (<[v:=InterT tv (ExT t)]> lty) cmd lty →
-          cmd_has_ty lty (CondTagC v t cmd) lty
-    .
-
-    Corollary CallTy_: ∀ lty lhs recv t targs name mdef args,
-      expr_has_ty lty recv (ClassT t targs) →
-      has_method name mdef t →
-      dom (gset string) mdef.(methodargs) = dom _ args →
-      (∀ x ty arg,
-      mdef.(methodargs) !! x = Some ty →
-      args !! x = Some arg →
-      ∃ ty', ty' <: subst_ty targs ty ∧ expr_has_ty lty arg ty') →
-      cmd_has_ty lty (CallC lhs recv name args) (<[lhs := subst_ty targs mdef.(methodrettype)]>lty).
-    Proof.
-      move => lty lhs recv t targs name mdef args hrecv hmdef hdom hargs.
-      econstructor; [done | done | done | ].
-      move => k ty arg hk ha.
-      destruct (hargs _ _ _ hk ha) as (ty' & hsub & he).
-      by econstructor.
-    Qed.
-
-    Lemma CallTyGen: ∀ lty lhs recv t targs name mdef args ret,
-      expr_has_ty lty recv (ClassT t targs) →
-      has_method name mdef t →
-      dom (gset string) mdef.(methodargs) = dom _ args →
-      (∀ x ty arg,
-      mdef.(methodargs) !! x = Some ty →
-      args !! x = Some arg →
-      ∃ ty', ty' <: subst_ty targs ty ∧ expr_has_ty lty arg ty') →
-      subst_ty targs mdef.(methodrettype) <: ret →
-      cmd_has_ty lty (CallC lhs recv name args) (<[lhs := ret]>lty).
-    Proof.
-      move =>lty lhs ?????? ret hrecv hm hdom hargs hret.
-      eapply SubTy; last by eapply CallTy_.
-      move => k A hA.
-      rewrite lookup_insert_Some in hA.
-      destruct hA as [[<- <-] | [hne heq]].
-      - rewrite lookup_insert.
-        by eexists.
-      - rewrite lookup_insert_ne //.
-        by exists A.
-    Qed.
-
-    Definition wf_mdef_ty t targs mdef :=
-      ∃ lty,
-      cmd_has_ty (<["$this" := ClassT t targs]>mdef.(methodargs)) mdef.(methodbody) lty ∧
-      expr_has_ty lty mdef.(methodret) mdef.(methodrettype)
-    .
-
-    Record wf_cdefs (prog: stringmap classDef)  := {
-      wf_fields : map_Forall (fun cname => wf_cdef_fields) prog;
-      wf_methods : map_Forall (fun cname => wf_cdef_methods) prog;
-      wf_mdefs :
-      map_Forall (fun cname cdef =>
-      map_Forall (fun mname mdef => wf_mdef_ty cname (gen_targs cdef.(generics)) mdef) cdef.(classmethods)) prog
+  Lemma mdef_incl_transitive: transitive _ mdef_incl.
+  Proof.
+    move => m0 m1 m2 [hdom1 [h1 ?]] [hdom2 [h2 ?]]; split; first by etransitivity.
+    split; last by eauto.
+    move => k A B hA hB.
+    destruct (methodargs m1 !! k) as [C | ] eqn:hC; last first.
+    { apply mk_is_Some in hA.
+      apply elem_of_dom in hA.
+      rewrite hdom1 in hA.
+      apply elem_of_dom in hA.
+      rewrite hC in hA.
+      by elim: hA.
     }
-    .
+    apply SubTrans with C.
+    - by eapply h2.
+    - by eapply h1.
+  Qed.
 
-    (* Big set reduction *)
-    Definition primop_eval (op: primop) : Z → Z → value :=
-      match op with
-      | PlusO => fun x y => IntV (x + y)
-      | MinusO => fun x y => IntV (x - y)
-      | TimesO => fun x y => IntV (x * y)
-      | DivO => fun x y => IntV (x / y)
-      | LeqO => fun x y => BoolV (Z.leb x y)
-      | GeqO => fun x y => BoolV (Z.geb x y)
-      | EqO => fun x y => BoolV (Z.eqb x y)
-      end
-    .
+  Definition wf_cdef_methods cdef : Prop :=
+    ∀ m mdef superdef super σ,
+    cdef.(superclass) = Some (super, σ) →
+    has_method m superdef super →
+    cdef.(classmethods) !! m = Some mdef →
+    mdef_incl mdef superdef.
 
-    Definition local_env := gmap var value.
+  Definition has_fields A (fields: stringmap (lang_ty * list lang_ty)) : Prop :=
+    ∀ fname typ inst, has_field fname A typ inst ↔ fields !! fname = Some (typ, inst).
 
-    Fixpoint expr_eval (le : local_env) (e: expr) : option value :=
-      match e with
-      | IntE z => Some (IntV z)
-      | BoolE b => Some (BoolV b)
-      | NullE => Some NullV
-      | OpE op e1 e2 =>
-          match expr_eval le e1, expr_eval le e2 with 
-          | Some (IntV z1), Some (IntV z2) => Some (primop_eval op z1 z2)
-          | _, _ => None
-          end
-      | VarE v => le !! v
-      end
-    .
+  Definition lift_fty (σ: list lang_ty) (fty: lang_ty * list lang_ty) :=
+    (fty.1, subst_ty σ <$> fty.2).
 
-    (* concrete heaps *)
-    Definition heap : Type := gmap loc (tag * stringmap value).
+  (*
+  Lemma has_method_fun: ∀ A name mdef0 mdef1,
+    has_method name mdef0 A → has_method name mdef1 A → mdef0 = mdef1.
+  Proof.
+    move => A name mdef0 mdef1 h; move: mdef1.
+    induction h as [ current cdef mdef hΔ hm 
+      | current parent inst cdef mdef hΔ hm hs hp hi ] => mdef1 h1.
+    - inv h1.
+      + rewrite hΔ in H; injection H; intros; subst; clear hΔ H.
+        rewrite hm in H0; injection H0; intros; by subst.
+      + rewrite hΔ in H; injection H; intros; subst; clear hΔ H.
+        rewrite hm in H0; discriminate H0.
+    - inv h1.
+      + rewrite hΔ in H; injection H; intros; subst; clear hΔ H.
+        rewrite hm in H0; discriminate H0.
+      + rewrite hΔ in H; injection H; intros; subst; clear hΔ H.
+        rewrite hs in H1; injection H1; intros; subst; clear hs H1.
+        apply hi in H2; by subst.
+  Qed.
+   *)
 
-    Definition map_args {A B: Type} (f: A → option  B) (m: stringmap A) :
-      option (stringmap B) :=
-      guard (map_Forall (λ _ x, is_Some (f x)) m); Some (omap f m)
-    .
+  Lemma has_field_inherits :
+    map_Forall (fun _ => wf_cdef_fields) Δ →
+    ∀ A B σ, inherits_using A B σ → 
+    ∀ f fty σf, has_field f B fty σf → has_field f A fty (subst_ty σ <$> σf).
+  Proof.
+    move => wfΔ A B σ h.
+    induction h as [ A B σ hext | A B σB C σC hAB hiAB hBC hiBC]; move => f fty σf hf.
+    - inv hext.
+      econstructor => //.
+      apply wfΔ in H.
+      by eapply H.
+    - apply hiBC in hf.
+      apply hiAB in hf.
+      by rewrite -map_subst_ty_subst.
+  Qed.
 
-    Lemma dom_map_args: ∀ A B (f: A → option B)
-      (m: stringmap A) (n: stringmap B),
-      map_args f m = Some n → 
-      dom stringset n = dom _ m.
-    Proof.
-      rewrite /map_args => A B f m n h.
-      case_option_guard; last done.
-      injection h; intros <-; clear h.
-      rewrite -> map_Forall_lookup in H.
-      apply set_eq => x; split; move/elem_of_dom => hx; apply elem_of_dom.
-      - rewrite lookup_omap in hx.
-        destruct hx as [v hv]; by apply bind_Some in hv as [a [-> ha]].
-      - destruct hx as [v hv].
-        rewrite lookup_omap hv.
-        by apply H in hv.
-    Qed.
+  Lemma has_fields_inherits :
+    map_Forall (fun _ => wf_cdef_fields) Δ →
+    ∀ A B σ, inherits_using A B σ → 
+    ∀ Afields Bfields, has_fields A Afields → has_fields B Bfields →
+    ∀ k fty σf, Bfields !! k = Some (fty, σf) →
+    Afields !! k = Some (fty, subst_ty σ <$> σf).
+  Proof.
+    move => wfΔ A B σ hin Afields Bfields hA hB k fty σf hk.
+    apply hB in hk.
+    apply has_field_inherits with (A := A) (σ := σ) in hk => //.
+    by apply hA.
+  Qed.
 
-    Lemma map_args_lookup: ∀ A B (f: A → option B) (m: stringmap A) n,
-      map_args f m = Some n →
-      ∀ k, n !! k = (m !! k) ≫= f.
-    Proof.
-      rewrite /map_args => A B f m n h k.
-      case_option_guard; last done.
-      injection h; intros <-; clear h.
-      rewrite -> map_Forall_lookup in H.
-      by rewrite lookup_omap.
-    Qed.
+  (*
 
-    Lemma map_args_empty: ∀ A B (f: A → option B),
-      map_args f ∅ = Some ∅.
-    Proof.
-      rewrite /map_args => A B f /=.
-      case_option_guard; first by rewrite omap_empty.
-      elim: H.
-      apply map_Forall_lookup => i x h; discriminate h.
-    Qed.
+  Corollary has_fields_inherits_lookup:
+    map_Forall (fun _ => wf_cdef_fields) Δ →
+    ∀ A B name fty fields,
+    has_field name fty B →
+    inherits A B →
+    has_fields A fields →
+    fields !! name = Some fty.
+  Proof.
+    move => wfΔ A B name fty fields hfields hinherits hf.
+    destruct (hf name fty) as [hl hr].
+    apply hl.
+    by eapply (has_field_inherits wfΔ).
+  Qed.
 
-    Lemma map_args_update: ∀ A B (f: A → option B) k a m n,
-      map_args f m = Some n →
-      map_args f (<[ k := a]> m) =
-      match f a with
-      | Some b => Some (<[ k := b]> n)
-      | None => None
-      end.
-    Proof.
-      rewrite /map_args => A B f k a m n h /=.
-      case_option_guard; last done.
-      injection h; intros <-; clear h.
-      case_option_guard.
-      - rewrite map_Forall_lookup in H0.
-        specialize H0 with k a.
-        rewrite lookup_insert in H0.
-        destruct H0 as [ b hb ]; first by done.
-        rewrite hb.
-        f_equal.
-        by apply omap_insert_Some.
-      - destruct (f a) as [b | ] eqn:hb; last done.
-        elim: H0 => i x h.
-        rewrite lookup_insert_Some in h.
-        destruct h as [[<- <-] | [hne hin]]; first by rewrite hb.
-        rewrite map_Forall_lookup in H.
-        now apply H in hin.
-    Qed.
+  Lemma has_method_inherits (Hcdef: map_Forall (fun _ => wf_cdef_methods) Δ):
+    ∀ A B, inherits A B →
+    ∀ m mdef, has_method m mdef B →
+    ∃ mdef', has_method m mdef' A ∧ mdef_incl mdef' mdef.
+  Proof.
+    move => A B h.
+    induction h as [ t | x y z hxy hyz hi]; move => m mdef hf.
+    { exists mdef; split => //.
+      by apply mdef_incl_reflexive.
+    }
+    apply hi in hf as (mdef' & hm & hincl).
+    destruct hxy as (cdef & hΔ & hs).
+    destruct (cdef.(classmethods) !! m) as [ mdef'' | ] eqn:heq; last first.
+    { exists mdef'; split; last done.
+      by apply InheritsMethod with y cdef.
+    }
+    exists mdef''; split; first by apply HasMethod with cdef.
+    apply mdef_incl_transitive with mdef'; last done.
+    apply Hcdef in hΔ.
+    by eapply hΔ.
+  Qed.
+   *)
 
-    Definition tag_match (st : local_env * heap) (v: string) (t: tag) :=
-      ∃ l, st.1 !! v = Some (LocV l) ∧
-      ∃ t' (fields: stringmap value), st.2 !! l = Some (t', fields) ∧
-      inherits t' t
-    .
+  (* Typing Judgements *)
+  Definition is_bool_op op : bool :=
+    match op with
+    | LeqO | GeqO | EqO => true
+    | PlusO | MinusO | TimesO | DivO => false
+    end
+  .
 
-    Inductive cmd_eval:
-      (local_env * heap) → cmd →
-      (local_env * heap) → nat → Prop :=
-      | SkipEv : ∀ st, cmd_eval st SkipC st 0
-      | LetEv: ∀ le h v e val,
-          expr_eval le e = Some val →
-          cmd_eval (le, h) (LetC v e) (<[v := val]> le, h) 0
-      (* targs are not stored in the heap: erased generics *)
-      | NewEv: ∀ le h lhs new t targs args vargs,
-          h !! new = None →
-          map_args (expr_eval le) args = Some vargs →
-          cmd_eval (le, h) (NewC lhs t targs args) (<[lhs := LocV new]>le, <[new := (t, vargs)]>h) 1
-      | GetEv: ∀ le h lhs recv name l t vs v,
-          expr_eval le recv = Some (LocV l) →
-          h !! l = Some (t, vs) →
-          vs !! name = Some v →
-          cmd_eval (le, h) (GetC lhs recv name) (<[lhs := v]>le, h) 1
-      | SetEv: ∀ le h recv fld rhs l v t vs vs',
-          expr_eval le recv = Some (LocV l) →
-          expr_eval le rhs = Some v →
-          h !! l = Some (t, vs) →
-          vs' = <[ fld := v ]>vs →
-          cmd_eval (le, h) (SetC recv fld rhs) (le, <[l := (t, vs')]> h) 0
-      | SeqEv: ∀ st1 st2 st3 fstc sndc n1 n2,
-          cmd_eval st1 fstc st2 n1 →
-          cmd_eval st2 sndc st3 n2 →
-          cmd_eval st1 (SeqC fstc sndc) st3 (n1 + n2)
-      | IfTrueEv: ∀ st1 st2 cond thn els n,
-          expr_eval st1.1 cond = Some (BoolV true) →
-          cmd_eval st1 thn st2 n →
-          cmd_eval st1 (IfC cond thn els) st2 n
-      | IfFalseEv: ∀ st1 st2 cond thn els n,
-          expr_eval st1.1 cond = Some (BoolV false) →
-          cmd_eval st1 els st2 n →
-          cmd_eval st1 (IfC cond thn els) st2 n
-      | CallEv: ∀ le h h' lhs recv l t vs name args vargs mdef
-          run_env run_env' ret n,
-          expr_eval le recv = Some (LocV l) →
-          map_args (expr_eval le) args = Some vargs →
-          h !! l = Some (t, vs) →
-          has_method name mdef t →
-          <["$this" := LocV l]>vargs = run_env →
-          cmd_eval (run_env, h) mdef.(methodbody) (run_env', h') n →
-          expr_eval run_env' mdef.(methodret) = Some ret →
-          cmd_eval (le, h) (CallC lhs recv name args) (<[lhs := ret]>le, h') (S n)
-      | CondTag1Ev n st1 st2 v t cmd :
-          (* tag in heap must <: requested tag to move forward *)
-          tag_match st1 v t →
-          cmd_eval st1 cmd st2 n →
-          cmd_eval st1 (CondTagC v t cmd) st2 n
-      | CondTag2Ev n st v t cmd :
-          ¬tag_match st v t →
-          cmd_eval st (CondTagC v t cmd) st n
+  Inductive expr_has_ty (lty : local_tys) :
+    expr → lang_ty → Prop :=
+    | IntTy : ∀ z, expr_has_ty lty (IntE z) IntT
+    | BoolTy: ∀ b, expr_has_ty lty (BoolE b) BoolT
+    | NullTy: expr_has_ty lty NullE NullT
+    | OpIntTy: ∀ op e1 e2,
+        is_bool_op op = false →
+        expr_has_ty lty e1 IntT →
+        expr_has_ty lty e2 IntT →
+        expr_has_ty lty (OpE op e1 e2) IntT
+    | OpBoolTy: ∀ op e1 e2,
+        is_bool_op op = true →
+        expr_has_ty lty e1 IntT →
+        expr_has_ty lty e2 IntT →
+        expr_has_ty lty (OpE op e1 e2) BoolT
+    | GenTy: ∀ v ty,
+        lty !! v = Some ty →
+        expr_has_ty lty (VarE v) ty
+    | ESubTy: ∀ e s t,
+        expr_has_ty lty e s →
+        s <: t →
+        expr_has_ty lty e t
+  .
+
+  (* continuation-based typing for commands *)
+  Inductive cmd_has_ty :
+    local_tys → cmd → local_tys → Prop :=
+    | SkipTy: ∀ lty, cmd_has_ty lty SkipC lty
+    | SeqTy: ∀ lty1 lty2 lty3 fstc sndc,
+        cmd_has_ty lty1 fstc lty2 →
+        cmd_has_ty lty2 sndc lty3 →
+        cmd_has_ty lty1 (SeqC fstc sndc) lty3
+    | LetTy: ∀ lty lhs e ty,
+        expr_has_ty lty e ty →
+        cmd_has_ty lty (LetC lhs e) (<[lhs := ty]>lty)
+    | IfTy: ∀ lty1 lty2 cond thn els,
+        expr_has_ty lty1 cond BoolT →
+        cmd_has_ty lty1 thn lty2 →
+        cmd_has_ty lty1 els lty2 →
+        cmd_has_ty lty1 (IfC cond thn els) lty2
+    | GetTy: ∀ lty lhs recv t σ σf name fty,
+        expr_has_ty lty recv (ClassT t σ) →
+        has_field name t fty σf →
+        cmd_has_ty lty (GetC lhs recv name) (<[lhs := subst_ty σ (subst_ty σf fty)]>lty)
+    | SetTy: ∀ lty recv fld rhs fty σf t σ,
+        expr_has_ty lty recv (ClassT t σ) →
+        has_field fld t fty σf →
+        expr_has_ty lty rhs (subst_ty σ (subst_ty σf fty)) →
+        cmd_has_ty lty (SetC recv fld rhs) lty
+        (*
+    | NewTy: ∀ lty lhs t targs args fields (*cdef*),
+        (* Δ !! t = Some cdef → *)
+        (* length targs = cdef.(generics) → (1* check constraints *1) *)
+        has_fields t fields →
+        dom (gset string) fields = dom _ args →
+        (∀ f fty arg,
+        fields !! f = Some fty →
+        args !! f = Some arg →
+        expr_has_ty lty arg (subst_ty targs fty)) →
+        cmd_has_ty lty (NewC lhs t args) (<[lhs := ClassT t targs]>lty)
+    | CallTy: ∀ lty lhs recv t targs name mdef args (*cdef*),
+        (* Δ !! t = Some cdef → *)
+        (* length targs = cdef.(generics) → *)
+        expr_has_ty lty recv (ClassT t targs) →
+        has_method name mdef t →
+        dom (gset string) mdef.(methodargs) = dom _ args →
+        (∀ x ty arg,
+        mdef.(methodargs) !! x = Some ty →
+        args !! x = Some arg →
+        expr_has_ty lty arg (subst_ty targs ty)) →
+        cmd_has_ty lty (CallC lhs recv name args) (<[lhs := subst_ty targs mdef.(methodrettype)]>lty)
+         *)
+    | SubTy: ∀ lty c rty rty',
+        rty' <:< rty →
+        cmd_has_ty lty c rty' →
+        cmd_has_ty lty c rty
+    | CondTagTy lty v tv t cmd :
+        lty !! v = Some tv →
+        cmd_has_ty (<[v:=InterT tv (ExT t)]> lty) cmd lty →
+        cmd_has_ty lty (CondTagC v t cmd) lty
+  .
+
+  (* TODO: update
+  Corollary CallTy_: ∀ lty lhs recv t targs name mdef args,
+    expr_has_ty lty recv (ClassT t targs) →
+    has_method name mdef t →
+    dom (gset string) mdef.(methodargs) = dom _ args →
+    (∀ x ty arg,
+    mdef.(methodargs) !! x = Some ty →
+    args !! x = Some arg →
+    ∃ ty', ty' <: subst_ty targs ty ∧ expr_has_ty lty arg ty') →
+    cmd_has_ty lty (CallC lhs recv name args) (<[lhs := subst_ty targs mdef.(methodrettype)]>lty).
+  Proof.
+    move => lty lhs recv t targs name mdef args hrecv hmdef hdom hargs.
+    econstructor; [done | done | done | ].
+    move => k ty arg hk ha.
+    destruct (hargs _ _ _ hk ha) as (ty' & hsub & he).
+    by econstructor.
+  Qed.
+
+  Lemma CallTyGen: ∀ lty lhs recv t targs name mdef args ret,
+    expr_has_ty lty recv (ClassT t targs) →
+    has_method name mdef t →
+    dom (gset string) mdef.(methodargs) = dom _ args →
+    (∀ x ty arg,
+    mdef.(methodargs) !! x = Some ty →
+    args !! x = Some arg →
+    ∃ ty', ty' <: subst_ty targs ty ∧ expr_has_ty lty arg ty') →
+    subst_ty targs mdef.(methodrettype) <: ret →
+    cmd_has_ty lty (CallC lhs recv name args) (<[lhs := ret]>lty).
+  Proof.
+    move =>lty lhs ?????? ret hrecv hm hdom hargs hret.
+    eapply SubTy; last by eapply CallTy_.
+    move => k A hA.
+    rewrite lookup_insert_Some in hA.
+    destruct hA as [[<- <-] | [hne heq]].
+    - rewrite lookup_insert.
+      by eexists.
+    - rewrite lookup_insert_ne //.
+      by exists A.
+  Qed.
+   *)
+
+  Definition subst_local_tys targs (lty: local_tys) : local_tys :=
+    (subst_ty targs) <$> lty.
+
+  Lemma dom_subst_local_tys targs lty :
+    dom stringset (subst_local_tys targs lty) = dom _ lty.
+  Proof. by rewrite /subst_local_tys dom_fmap_L. Qed.
+
+  Lemma lookup_subst_local_tys targs lty k:
+    (subst_local_tys targs lty) !! k = subst_ty targs <$> lty !! k.
+  Proof. by rewrite /subst_local_tys lookup_fmap. Qed.
+
+  Lemma lookup_subst_local_tys_Some targs lty k ty:
+    (subst_local_tys targs lty) !! k = Some ty →
+    ∃ ty', lty !! k = Some ty' ∧ ty = subst_ty targs ty'.
+  Proof.
+    rewrite lookup_subst_local_tys.
+    destruct (lty !! k) as [ ty' | ] eqn:h => //=.
+    case => <-.
+    by exists ty'.
+  Qed.
+
+  Lemma insert_subst_local_tys targs lhs ty lty:
+    subst_local_tys targs (<[lhs:=ty]> lty) =
+    <[lhs := subst_ty targs ty]>(subst_local_tys targs lty).
+  Proof. by rewrite /subst_local_tys fmap_insert. Qed.
+
+  Lemma subst_local_tys_gen_targs_is_bounded n lty:
+    map_Forall (λ _ ty, bounded n ty) lty →
+    subst_local_tys (gen_targs n) lty = lty.
+  Proof.
+    move => h.
+    apply map_eq => k.
+    rewrite lookup_subst_local_tys.
+    rewrite map_Forall_lookup in h.
+    destruct (lty !! k) as [ty | ] eqn:hty => //=.
+    rewrite hty.
+    apply h in hty.
+    by rewrite subst_gen_targs_is_bounded.
+  Qed.
+
+  Lemma lty_sub_subst lty rty:
+    lty <:< rty →
+    ∀ targs, (subst_local_tys targs lty) <:< (subst_local_tys targs rty).
+  Proof.
+    rewrite /lty_sub => h targs k A.
+    rewrite !lookup_subst_local_tys.
+    destruct (rty !! k) as [ty | ] eqn:hty; last done.
+    move => /= [<-].
+    apply h in hty as [B [-> hsub]].
+    exists (subst_ty targs B); split; first done.
+    by apply subtype_subst.
+  Qed.
+
+  Lemma expr_has_ty_subst lty e ty:
+    expr_has_ty lty e ty →
+    ∀ targs,
+    expr_has_ty (subst_local_tys targs lty) e (subst_ty targs ty).
+  Proof.
+    induction 1 as [ z | b | | op e1 e2 hop h1 hi1 h2 hi2
+      | op e1 e2 hop h1 hi1 h2 hi2 | v ty hv
+      | e s t hs hi hsub ] => targs; try by constructor.
+    - simpl in *; by constructor.
+    - simpl in *; by constructor.
+    - constructor.
+      by rewrite /subst_local_tys lookup_fmap hv.
+    - econstructor; first by apply hi.
+      by apply subtype_subst.
+  Qed.
+
+  (* Consider a class C<T0, ..., Tn>,
+     method bodies are checked under a generic env = [| T0, .., Tn |]
+   *)
+  Definition wf_mdef_ty t n mdef :=
+    let targs := gen_targs n in
+    ∃ lty,
+    cmd_has_ty (<["$this" := ClassT t targs]>(subst_local_tys targs mdef.(methodargs))) mdef.(methodbody) lty ∧
+    expr_has_ty lty mdef.(methodret) (subst_ty targs mdef.(methodrettype))
+  .
+
+  Record wf_cdefs (prog: stringmap classDef) := {
+    wf_fields : map_Forall (λ _cname, wf_cdef_fields) prog;
+    wf_fields_bounded : map_Forall (λ _cname, wf_cdef_fields_bounded) prog;
+    wf_methods : map_Forall (λ _cname, wf_cdef_methods) prog;
+    wf_methods_bounded : map_Forall (λ _cname, cdef_methods_bounded) prog;
+    wf_mdefs :
+      map_Forall (λ cname cdef,
+        map_Forall (λ _mname mdef,
+           wf_mdef_ty cname cdef.(generics) mdef)
+        cdef.(classmethods)) prog
+  }
+  .
+
+  (* Big step reduction *)
+  Definition primop_eval (op: primop) : Z → Z → value :=
+    match op with
+    | PlusO => fun x y => IntV (x + y)
+    | MinusO => fun x y => IntV (x - y)
+    | TimesO => fun x y => IntV (x * y)
+    | DivO => fun x y => IntV (x / y)
+    | LeqO => fun x y => BoolV (Z.leb x y)
+    | GeqO => fun x y => BoolV (Z.geb x y)
+    | EqO => fun x y => BoolV (Z.eqb x y)
+    end
+  .
+
+  Definition local_env := gmap var value.
+
+  Fixpoint expr_eval (le : local_env) (e: expr) : option value :=
+    match e with
+    | IntE z => Some (IntV z)
+    | BoolE b => Some (BoolV b)
+    | NullE => Some NullV
+    | OpE op e1 e2 =>
+        match expr_eval le e1, expr_eval le e2 with 
+        | Some (IntV z1), Some (IntV z2) => Some (primop_eval op z1 z2)
+        | _, _ => None
+        end
+    | VarE v => le !! v
+    end
+  .
+
+  (* concrete heaps *)
+  Definition heap : Type := gmap loc (tag * stringmap value).
+
+  Definition map_args {A B: Type} (f: A → option  B) (m: stringmap A) :
+    option (stringmap B) :=
+    guard (map_Forall (λ _ x, is_Some (f x)) m); Some (omap f m)
+  .
+
+  Lemma dom_map_args: ∀ A B (f: A → option B)
+    (m: stringmap A) (n: stringmap B),
+    map_args f m = Some n → 
+    dom stringset n = dom _ m.
+  Proof.
+    rewrite /map_args => A B f m n h.
+    case_option_guard; last done.
+    injection h; intros <-; clear h.
+    rewrite -> map_Forall_lookup in H.
+    apply set_eq => x; split; move/elem_of_dom => hx; apply elem_of_dom.
+    - rewrite lookup_omap in hx.
+      destruct hx as [v hv]; by apply bind_Some in hv as [a [-> ha]].
+    - destruct hx as [v hv].
+      rewrite lookup_omap hv.
+      by apply H in hv.
+  Qed.
+
+  Lemma map_args_lookup: ∀ A B (f: A → option B) (m: stringmap A) n,
+    map_args f m = Some n →
+    ∀ k, n !! k = (m !! k) ≫= f.
+  Proof.
+    rewrite /map_args => A B f m n h k.
+    case_option_guard; last done.
+    injection h; intros <-; clear h.
+    rewrite -> map_Forall_lookup in H.
+    by rewrite lookup_omap.
+  Qed.
+
+  Lemma map_args_empty: ∀ A B (f: A → option B),
+    map_args f ∅ = Some ∅.
+  Proof.
+    rewrite /map_args => A B f /=.
+    case_option_guard; first by rewrite omap_empty.
+    elim: H.
+    apply map_Forall_lookup => i x h; discriminate h.
+  Qed.
+
+  Lemma map_args_update: ∀ A B (f: A → option B) k a m n,
+    map_args f m = Some n →
+    map_args f (<[ k := a]> m) =
+    match f a with
+    | Some b => Some (<[ k := b]> n)
+    | None => None
+    end.
+  Proof.
+    rewrite /map_args => A B f k a m n h /=.
+    case_option_guard; last done.
+    injection h; intros <-; clear h.
+    case_option_guard.
+    - rewrite map_Forall_lookup in H0.
+      specialize H0 with k a.
+      rewrite lookup_insert in H0.
+      destruct H0 as [ b hb ]; first by done.
+      rewrite hb.
+      f_equal.
+      by apply omap_insert_Some.
+    - destruct (f a) as [b | ] eqn:hb; last done.
+      elim: H0 => i x h.
+      rewrite lookup_insert_Some in h.
+      destruct h as [[<- <-] | [hne hin]]; first by rewrite hb.
+      rewrite map_Forall_lookup in H.
+      now apply H in hin.
+  Qed.
+
+  Definition tag_match (st : local_env * heap) (v: string) (t: tag) :=
+    ∃ l, st.1 !! v = Some (LocV l) ∧
+    ∃ t' (fields: stringmap value), st.2 !! l = Some (t', fields) ∧
+    inherits t' t
+  .
+
+  Inductive cmd_eval:
+    (local_env * heap) → cmd →
+    (local_env * heap) → nat → Prop :=
+    | SkipEv : ∀ st, cmd_eval st SkipC st 0
+    | LetEv: ∀ le h v e val,
+        expr_eval le e = Some val →
+        cmd_eval (le, h) (LetC v e) (<[v := val]> le, h) 0
+    (* targs are not stored in the heap: erased generics *)
+    | NewEv: ∀ le h lhs new t args vargs,
+        h !! new = None →
+        map_args (expr_eval le) args = Some vargs →
+        cmd_eval (le, h) (NewC lhs t args) (<[lhs := LocV new]>le, <[new := (t, vargs)]>h) 1
+    | GetEv: ∀ le h lhs recv name l t vs v,
+        expr_eval le recv = Some (LocV l) →
+        h !! l = Some (t, vs) →
+        vs !! name = Some v →
+        cmd_eval (le, h) (GetC lhs recv name) (<[lhs := v]>le, h) 1
+    | SetEv: ∀ le h recv fld rhs l v t vs vs',
+        expr_eval le recv = Some (LocV l) →
+        expr_eval le rhs = Some v →
+        h !! l = Some (t, vs) →
+        vs' = <[ fld := v ]>vs →
+        cmd_eval (le, h) (SetC recv fld rhs) (le, <[l := (t, vs')]> h) 0
+    | SeqEv: ∀ st1 st2 st3 fstc sndc n1 n2,
+        cmd_eval st1 fstc st2 n1 →
+        cmd_eval st2 sndc st3 n2 →
+        cmd_eval st1 (SeqC fstc sndc) st3 (n1 + n2)
+    | IfTrueEv: ∀ st1 st2 cond thn els n,
+        expr_eval st1.1 cond = Some (BoolV true) →
+        cmd_eval st1 thn st2 n →
+        cmd_eval st1 (IfC cond thn els) st2 n
+    | IfFalseEv: ∀ st1 st2 cond thn els n,
+        expr_eval st1.1 cond = Some (BoolV false) →
+        cmd_eval st1 els st2 n →
+        cmd_eval st1 (IfC cond thn els) st2 n
+    | CallEv: ∀ le h h' lhs recv l t vs name args vargs mdef
+        run_env run_env' ret n,
+        expr_eval le recv = Some (LocV l) →
+        map_args (expr_eval le) args = Some vargs →
+        h !! l = Some (t, vs) →
+        has_method name mdef t →
+        <["$this" := LocV l]>vargs = run_env →
+        cmd_eval (run_env, h) mdef.(methodbody) (run_env', h') n →
+        expr_eval run_env' mdef.(methodret) = Some ret →
+        cmd_eval (le, h) (CallC lhs recv name args) (<[lhs := ret]>le, h') (S n)
+    | CondTag1Ev n st1 st2 v t cmd :
+        (* tag in heap must <: requested tag to move forward *)
+        tag_match st1 v t →
+        cmd_eval st1 cmd st2 n →
+        cmd_eval st1 (CondTagC v t cmd) st2 n
+    | CondTag2Ev n st v t cmd :
+        ¬tag_match st v t →
+        cmd_eval st (CondTagC v t cmd) st n
 .
+
 End ProgDef.
 
 (* Hints and notations are local to the section. Re-exporting them *)
 Global Hint Constructors subtype : core.
 Global Hint Constructors has_field : core.
-Global Hint Constructors has_method : code.
+Global Hint Constructors has_method : core.
